SeparationLogic/Complete/ContextProperty_Flat.v
@@ -1,0 +1,134 @@
+Require Import Logic.GeneralLogic.Base.
+Require Import Logic.GeneralLogic.HenkinCompleteness.
+Require Import Logic.MinimunLogic.Syntax.
+Require Import Logic.PropositionalLogic.Syntax.
+Require Import Logic.SeparationLogic.Syntax.
+Require Import Logic.MinimunLogic.ProofTheory.Normal.
+Require Import Logic.MinimunLogic.ProofTheory.Minimun.
+Require Import Logic.MinimunLogic.ProofTheory.ContextProperty.
+Require Import Logic.PropositionalLogic.ProofTheory.Intuitionistic.
+Require Import Logic.PropositionalLogic.ProofTheory.DeMorgan.
+Require Import Logic.PropositionalLogic.ProofTheory.GodelDummett.
+Require Import Logic.PropositionalLogic.ProofTheory.Classical.
+Require Import Logic.PropositionalLogic.ProofTheory.RewriteClass.
+Require Import Logic.SeparationLogic.ProofTheory.SeparationLogic.
+Require Import Logic.SeparationLogic.ProofTheory.RewriteClass.
+Require Import Logic.SeparationLogic.ProofTheory.DerivedRules.
+
+Local Open Scope logic_base.
+Local Open Scope syntax.
+Import PropositionalLanguageNotation.
+Import SeparationLogicNotation.
+
+Definition context_join {L: Language} {sL: SeparationLanguage L} {Gamma: ProofTheory L} (Phi1 Phi2 Phi: context): Prop :=
+  forall x y, Phi1 |-- x -> Phi2 |-- y -> Phi |-- x * y.
+
+Definition context_sepcon {L: Language} {sL: SeparationLanguage L} {Gamma: ProofTheory L} (Phi Psi: context): context :=
+  fun z => exists x y, z = x * y /\ Phi |-- x /\ Psi |-- y.
+
+Definition Linderbaum_sepcon_right
+           {L: Language}
+           {sL: SeparationLanguage L}
+           {Gamma: ProofTheory L}
+           (P: context -> Prop): Prop :=
+  forall (Phi1 Phi2: context) (Psi: sig P),
+    context_join Phi1 Phi2 (proj1_sig Psi) ->
+    exists Psi2: sig P,
+      Included _ Phi2 (proj1_sig Psi2) /\
+      context_join Phi1 (proj1_sig Psi2) (proj1_sig Psi).
+
+Definition Linderbaum_sepcon_left
+           {L: Language}
+           {sL: SeparationLanguage L}
+           {Gamma: ProofTheory L}
+           (P: context -> Prop): Prop :=
+  forall (Phi1 Phi2: context) (Psi: sig P),
+    context_join Phi1 Phi2 (proj1_sig Psi) ->
+    exists Psi1: sig P,
+      Included _ Phi1 (proj1_sig Psi1) /\
+      context_join (proj1_sig Psi1) Phi2 (proj1_sig Psi).
+
+Lemma context_sepcon_context_join {L: Language} {nL: NormalLanguage L} {sL: SeparationLanguage L} {Gamma: ProofTheory L} {nGamma: NormalProofTheory L Gamma} {mpGamma: MinimunPropositionalLogic L Gamma}:
+  forall Phi1 Phi2,
+    context_join Phi1 Phi2 (context_sepcon Phi1 Phi2).
+Proof.
+  intros.
+  hnf; intros.
+  apply derivable_assum.
+  exists x, y.
+  auto.
+Qed.
+
+Lemma context_sepcon_context_join' {L: Language} {nL: NormalLanguage L} {sL: SeparationLanguage L} {Gamma: ProofTheory L} {nGamma: NormalProofTheory L Gamma} {mpGamma: MinimunPropositionalLogic L Gamma}:
+  forall Phi1 Phi2 Phi,
+    Included _ (context_sepcon Phi1 Phi2) Phi ->
+    context_join Phi1 Phi2 Phi.
+Proof.
+  intros.
+  hnf; intros.
+  apply derivable_assum, H.
+  exists x, y.
+  auto.
+Qed.
+
+Lemma context_sepcon_derivable {L: Language} {nL: NormalLanguage L} {pL: PropositionalLanguage L} {sL: SeparationLanguage L} {Gamma: ProofTheory L} {nGamma: NormalProofTheory L Gamma} {mpGamma: MinimunPropositionalLogic L Gamma} {ipGamma: IntuitionisticPropositionalLogic L Gamma} {sGamma: SeparationLogic L Gamma}:
+  forall (Phi Psi: context) z,
+    context_sepcon Phi Psi |-- z ->
+    exists x y, |-- x * y --> z /\ Phi |-- x /\ Psi |-- y.
+Proof.
+  intros.
+  rewrite derivable_provable in H.
+  destruct H as [xs [? ?]].
+  revert z H0; induction H; intros.
+  + exists TT, TT.
+    split; [| split].
+    - apply aux_minimun_rule00; auto.
+    - apply derivable_impp_refl.
+    - apply derivable_impp_refl.
+  + pose proof provable_multi_imp_arg_switch1 l x z.
+    pose proof modus_ponens _ _ H2 H1.
+    specialize (IHForall _ H3); clear H1 H2 H3.
+    destruct H as [x' [y' [? [? ?]]]]; subst x.
+    destruct IHForall as [x [y [? [? ?]]]].
+    exists (x && x'), (y && y').
+    split; [| split].
+    - clear l H0 H1 H2 H3 H4.
+      rewrite (provable_sepcon_andp_right (x && x') y y').
+      rewrite (provable_sepcon_andp_left x x' y).
+      rewrite (provable_sepcon_andp_left x x' y').
+      rewrite (andp_elim1 (x * y) _).
+      rewrite (andp_elim2 _ (x' * y')).
+      rewrite provable_derivable.
+      rewrite <- deduction_theorem.
+      pose proof derivable_assum1 empty_context ((x * y) && (x' * y')).
+      pose proof deduction_andp_elim1 _ _ _ H0.
+      pose proof deduction_andp_elim2 _ _ _ H0.
+      apply (deduction_weaken0 (Union _ empty_context (Singleton _ (x * y && (x' * y'))))) in H.
+      pose proof deduction_modus_ponens _ _ _ H1 H.
+      pose proof deduction_modus_ponens _ _ _ H2 H3.
+      auto.
+    - apply deduction_andp_intros; auto.
+    - apply deduction_andp_intros; auto.
+Qed.
+
+Lemma wand_deduction_theorem {L: Language} {nL: NormalLanguage L} {pL: PropositionalLanguage L} {sL: SeparationLanguage L} {Gamma: ProofTheory L} {nGamma: NormalProofTheory L Gamma} {mpGamma: MinimunPropositionalLogic L Gamma} {ipGamma: IntuitionisticPropositionalLogic L Gamma} {sGamma: SeparationLogic L Gamma}:
+  forall (Phi: context) x y,
+    context_sepcon Phi (Union _ empty_context (Singleton _ x)) |-- y <->
+    Phi |-- x -* y.
+Proof.
+  intros.
+  split; intros.
+  + apply context_sepcon_derivable in H.
+    destruct H as [x' [y' [? [? ?]]]].
+    rewrite deduction_theorem, <- provable_derivable in H1.
+    rewrite <- H1 in H.
+    apply wand_sepcon_adjoint in H.
+    rewrite H in H0; auto.
+  + rewrite <- (provable_wand_sepcon_modus_ponens1 x y).
+    apply derivable_assum.
+    exists (x -* y), x.
+    split; [| split]; auto.
+    rewrite deduction_theorem.
+    apply derivable_impp_refl.
+Qed.
+
