SeparationLogic/Complete/Truth_Flat.v
@@ -1,0 +1,162 @@
+Require Import Coq.Logic.Classical_Prop.
+Require Import Coq.Logic.Classical_Pred_Type.
+Require Import Logic.lib.Bijection.
+Require Import Logic.lib.Countable.
+Require Import Logic.GeneralLogic.Base.
+Require Import Logic.GeneralLogic.HenkinCompleteness.
+Require Import Logic.MinimunLogic.Syntax.
+Require Import Logic.PropositionalLogic.Syntax.
+Require Import Logic.SeparationLogic.Syntax.
+Require Import Logic.MinimunLogic.ProofTheory.Normal.
+Require Import Logic.MinimunLogic.ProofTheory.Minimun.
+Require Import Logic.MinimunLogic.ProofTheory.ContextProperty.
+Require Import Logic.PropositionalLogic.ProofTheory.Intuitionistic.
+Require Import Logic.PropositionalLogic.ProofTheory.DeMorgan.
+Require Import Logic.PropositionalLogic.ProofTheory.GodelDummett.
+Require Import Logic.PropositionalLogic.ProofTheory.Classical.
+Require Import Logic.PropositionalLogic.ProofTheory.RewriteClass.
+Require Import Logic.SeparationLogic.ProofTheory.SeparationLogic.
+Require Import Logic.SeparationLogic.ProofTheory.RewriteClass.
+Require Import Logic.SeparationLogic.ProofTheory.DerivedRules.
+Require Import Logic.GeneralLogic.KripkeModel.
+Require Import Logic.SeparationLogic.Model.SeparationAlgebra.
+Require Import Logic.SeparationLogic.Model.OrderedSA.
+Require Import Logic.PropositionalLogic.Semantics.Kripke.
+Require Import Logic.SeparationLogic.Semantics.FlatSemantics.
+Require Import Logic.PropositionalLogic.Complete.ContextProperty_Kripke.
+Require Import Logic.SeparationLogic.Complete.ContextProperty_Flat.
+
+Local Open Scope logic_base.
+Local Open Scope syntax.
+Local Open Scope kripke_model.
+Import PropositionalLanguageNotation.
+Import SeparationLogicNotation.
+Import KripkeModelFamilyNotation.
+Import KripkeModelNotation_Intuitionistic.
+
+Section TruthLemma.
+
+Context {L: Language}
+        {nL: NormalLanguage L}
+        {pL: PropositionalLanguage L}
+        {sL: SeparationLanguage L}
+        {Gamma: ProofTheory L}
+        {nGamma: NormalProofTheory L Gamma}
+        {mpGamma: MinimunPropositionalLogic L Gamma}
+        {ipGamma: IntuitionisticPropositionalLogic L Gamma}
+        {sGamma: SeparationLogic L Gamma}
+        {MD: Model}
+        {kMD: KripkeModel MD}
+        {M: Kmodel}
+        {R: Relation (Kworlds M)}
+        {J: Join (Kworlds M)}
+        {SM: Semantics L MD}
+        {kpSM: KripkePropositionalSemantics L MD M SM}
+        {fsSM: SeparatingSemantics L MD M SM}.
+
+Context (P: context -> Prop)
+        (rel: bijection (Kworlds M) (sig P)).
+
+Hypothesis H_R: forall m n Phi Psi, rel m Phi -> rel n Psi -> (m <= n <-> Included _ (proj1_sig Phi) (proj1_sig Psi)).
+
+Hypothesis H_J: forall m1 m2 m Phi1 Phi2 Phi, rel m1 Phi1 -> rel m2 Phi2 -> rel m Phi -> (join m1 m2 m <-> context_join (proj1_sig Phi1) (proj1_sig Phi2) (proj1_sig Phi)).
+
+Lemma truth_lemma_sepcon
+      (DER: at_least_derivable_closed P)
+      (LIN_SL: Linderbaum_sepcon_left P)
+      (LIN_SR: Linderbaum_sepcon_right P)
+      (x y: expr)
+      (IHx: forall m Phi, rel m Phi -> (KRIPKE: M, m |= x <-> proj1_sig Phi x))
+      (IHy: forall m Phi, rel m Phi -> (KRIPKE: M, m |= y <-> proj1_sig Phi y)):
+  forall m Phi, rel m Phi -> (KRIPKE: M, m |= x * y <-> proj1_sig Phi (x * y)).
+Proof.
+  intros.
+  rewrite sat_sepcon.
+  split; intros.
+  + destruct H0 as [m1 [m2 [? [? ?]]]].
+    destruct (im_bij _ _ rel m1) as [Phi1 ?].
+    destruct (im_bij _ _ rel m2) as [Phi2 ?].
+    erewrite IHx in H1 by eauto.
+    erewrite IHy in H2 by eauto.
+    erewrite H_J in H0 by eauto.
+    rewrite derivable_closed_element_derivable by (apply DER, (proj2_sig Phi)).
+    apply H0.
+    - rewrite <- derivable_closed_element_derivable by (apply DER, (proj2_sig Phi1)); auto.
+    - rewrite <- derivable_closed_element_derivable by (apply DER, (proj2_sig Phi2)); auto.
+  + rewrite derivable_closed_element_derivable in H0 by (apply DER, (proj2_sig Phi)).
+    assert (context_join (Union _ empty_context (Singleton _ x))
+             (Union _ empty_context (Singleton _ y)) (proj1_sig Phi)).
+    Focus 1. {
+      hnf; intros.
+      rewrite deduction_theorem, <- provable_derivable in H1, H2.
+      rewrite <- H1, <- H2.
+      auto.
+    } Unfocus.
+    apply LIN_SL in H1.
+    destruct H1 as [Phi1 [? ?]].
+    apply LIN_SR in H2.
+    destruct H2 as [Phi2 [? ?]].
+    destruct (su_bij _ _ rel Phi1) as [m1 ?].
+    destruct (su_bij _ _ rel Phi2) as [m2 ?].
+    exists m1, m2.
+    erewrite H_J, IHx, IHy by eauto.
+    split; [| split]; auto.
+    - apply H1; right; constructor.
+    - apply H2; right; constructor.
+Qed.
+
+Lemma truth_lemma_wand
+      (DER: at_least_derivable_closed P)
+      (LIN_DER: Linderbaum_derivable P)
+      (LIN_SR: Linderbaum_sepcon_right P)
+      (x y: expr)
+      (IHx: forall m Phi, rel m Phi -> (KRIPKE: M, m |= x <-> proj1_sig Phi x))
+      (IHy: forall m Phi, rel m Phi -> (KRIPKE: M, m |= y <-> proj1_sig Phi y)):
+  forall m Phi, rel m Phi -> (KRIPKE: M, m |= x -* y <-> proj1_sig Phi (x -* y)).
+Proof.
+  intros.
+  rewrite sat_wand.
+  split; intros.
+  + rewrite derivable_closed_element_derivable by (apply DER, (proj2_sig Phi)); auto.
+    rewrite <- wand_deduction_theorem.
+    apply NNPP; intro.
+    apply LIN_DER in H1.
+    destruct H1 as [Phi2 [? ?]].
+    apply context_sepcon_context_join' in H1.
+    apply H2; clear H2.
+    rewrite <- derivable_closed_element_derivable by (apply DER, (proj2_sig Phi2)); auto.
+    apply LIN_SR in H1.
+    destruct H1 as [Phi1 [? ?]].
+    destruct (su_bij _ _ rel Phi1) as [m1 ?].
+    destruct (su_bij _ _ rel Phi2) as [m2 ?].
+    erewrite <- IHy by eauto.
+    erewrite <- H_J in H2 by eauto.
+    apply (H0 _ _ H2).
+    erewrite IHx by eauto.
+    apply H1; right; constructor.
+  + destruct (im_bij _ _ rel m1) as [Phi1 ?].
+    destruct (im_bij _ _ rel m2) as [Phi2 ?].
+    erewrite IHy by eauto.
+    erewrite IHx in H2 by eauto.
+    erewrite H_J in H1 by eauto.
+    rewrite derivable_closed_element_derivable in H0 by (apply DER, (proj2_sig Phi)).
+    rewrite derivable_closed_element_derivable in H2 by (apply DER, (proj2_sig Phi1)).
+    rewrite derivable_closed_element_derivable by (apply DER, (proj2_sig Phi2)).
+    specialize (H1 _ _ H0 H2).
+    rewrite provable_wand_sepcon_modus_ponens1 in H1; auto.
+Qed.
+(*
+Lemma truth_lemma_emp:
+  forall m Phi, rel m Phi -> (KRIPKE: M, m |= emp <-> proj1_sig Phi emp).
+Proof.
+  intros.
+  rewrite sat_falsep.
+  pose proof proj2_sig Phi.
+  pose proof CONSI _ H0.
+  rewrite consistent_spec in H1.
+  split; [intros [] |].
+  intro; apply H1.
+  apply derivable_assum; auto.
+Qed.
+*)
+End TruthLemma.
